<?xml version="1.0" encoding="UTF-8"?>
<rdf:RDF xmlns:rdf="http://www.w3.org/1999/02/22-rdf-syntax-ns#">
  <skos:ConceptScheme xmlns:skos="http://www.w3.org/2004/02/skos/core#" rdf:about="http://inspire.ec.europa.eu/metadata-codelist/SpatialScope">
    <dc:title xmlns:dc="http://purl.org/dc/elements/1.1/">Spatial scope</dc:title>
    <dc:description xmlns:dc="http://purl.org/dc/elements/1.1/" xml:lang="en">Administrative level that the data set intends to cover.</dc:description>
    <dcterms:issued xmlns:dcterms="http://purl.org/dc/terms/">2019-05-22</dcterms:issued>
    <dcterms:modified xmlns:dcterms="http://purl.org/dc/terms/">2019-05-22</dcterms:modified>
  </skos:ConceptScheme>
  <skos:Concept xmlns:skos="http://www.w3.org/2004/02/skos/core#" rdf:about="http://inspire.ec.europa.eu/metadata-codelist/SpatialScope/national">
    <skos:prefLabel xml:lang="en">National</skos:prefLabel>
    <skos:scopeNote xml:lang="en">The scope of the data set intends to cover the national territory.</skos:scopeNote>
    <skos:prefLabel xml:lang="bg">Национално ниво</skos:prefLabel>
    <skos:scopeNote xml:lang="bg">Обхватът на набора от данни има за цел да покрие националната територия.</skos:scopeNote>
    <skos:prefLabel xml:lang="cs">Národní</skos:prefLabel>
    <skos:scopeNote xml:lang="cs">Datová sada má v úmyslu pokrýt území státu.</skos:scopeNote>
    <skos:prefLabel xml:lang="hr">Nacionalni</skos:prefLabel>
    <skos:scopeNote xml:lang="hr">Opseg skupa podataka namjerava se odnositi na nacionalno područje.</skos:scopeNote>
    <skos:prefLabel xml:lang="da">National</skos:prefLabel>
    <skos:scopeNote xml:lang="da">Formålet med datasættet er at dække det nationale område.</skos:scopeNote>
    <skos:prefLabel xml:lang="de">National</skos:prefLabel>
    <skos:scopeNote xml:lang="de">Der Geltungsbereich des Datensatzes deckt das nationale Hoheitsgebiet ab.</skos:scopeNote>
    <skos:prefLabel xml:lang="el">Εθνικό</skos:prefLabel>
    <skos:scopeNote xml:lang="el">Το πεδίο εφαρμογής του συνόλου δεδομένων έχει ως στόχο να καλύπτει την εθνική επικράτεια.</skos:scopeNote>
    <skos:prefLabel xml:lang="es">Nacional</skos:prefLabel>
    <skos:scopeNote xml:lang="es">El ámbito de aplicación del conjunto de datos se propone cubrir el territorio nacional.</skos:scopeNote>
    <skos:prefLabel xml:lang="et">Riiklik</skos:prefLabel>
    <skos:scopeNote xml:lang="et">Andmekogumi eesmärk on hõlmata riigi territoorium.</skos:scopeNote>
    <skos:prefLabel xml:lang="fi">Kansallinen</skos:prefLabel>
    <skos:scopeNote xml:lang="fi">Tietoaineiston tarkoituksena on kattaa kansallinen alue.</skos:scopeNote>
    <skos:prefLabel xml:lang="fr">National</skos:prefLabel>
    <skos:scopeNote xml:lang="fr">Le champ d’application de la série de données vise à couvrir le territoire national.</skos:scopeNote>
    <skos:prefLabel xml:lang="hu">Nemzeti</skos:prefLabel>
    <skos:scopeNote xml:lang="hu">Az adatkészlet terjedelme az ország területét érinti.</skos:scopeNote>
    <skos:prefLabel xml:lang="it">Nazionale</skos:prefLabel>
    <skos:scopeNote xml:lang="it">L'ambito di applicazione dell'insieme di dati è esteso al territorio nazionale.</skos:scopeNote>
    <skos:prefLabel xml:lang="lt">Nacionalinės</skos:prefLabel>
    <skos:scopeNote xml:lang="lt">Duomenų rinkinio taikymo sritis apima ir nacionalinę teritoriją.</skos:scopeNote>
    <skos:prefLabel xml:lang="lv">Valsts</skos:prefLabel>
    <skos:scopeNote xml:lang="lv">Datu kopas darbības joma ir paredzēta, lai aptvertu valsts teritoriju.</skos:scopeNote>
    <skos:prefLabel xml:lang="mt">Nazzjonali</skos:prefLabel>
    <skos:scopeNote xml:lang="mt">Il-kamp ta’ applikazzjoni tas-sett ta’ dejta għandu l-għan li jkopri t-territorju nazzjonali.</skos:scopeNote>
    <skos:prefLabel xml:lang="nl">Nationaal</skos:prefLabel>
    <skos:scopeNote xml:lang="nl">De reikwijdte van de gegevensverzameling is bedoeld om het nationale grondgebied te bestrijken.</skos:scopeNote>
    <skos:prefLabel xml:lang="pl">Krajowe</skos:prefLabel>
    <skos:scopeNote xml:lang="pl">Zakres zbioru danych ma obejmować terytorium krajowe.</skos:scopeNote>
    <skos:prefLabel xml:lang="pt">Nacional</skos:prefLabel>
    <skos:scopeNote xml:lang="pt">O âmbito do conjunto de dados pretende abranger o território nacional.</skos:scopeNote>
    <skos:prefLabel xml:lang="ro">Național</skos:prefLabel>
    <skos:scopeNote xml:lang="ro">Domeniul de aplicare al setului de date vizează acoperirea teritoriului național.</skos:scopeNote>
    <skos:prefLabel xml:lang="sk">Národný</skos:prefLabel>
    <skos:scopeNote xml:lang="sk">Rozsah súboru priestorových údajov sa vzťahuje na územie štátu.</skos:scopeNote>
    <skos:prefLabel xml:lang="sl">Nacionalno</skos:prefLabel>
    <skos:scopeNote xml:lang="sl">Namen zbirke podatkov je zajeti nacionalno ozemlje.</skos:scopeNote>
    <skos:prefLabel xml:lang="sv">Nationell</skos:prefLabel>
    <skos:scopeNote xml:lang="sv">Syftet med datamängden är att täcka in det nationella territoriet.</skos:scopeNote>
    <skos:inScheme rdf:resource="http://inspire.ec.europa.eu/metadata-codelist/SpatialScope" />
  </skos:Concept>
  <skos:Concept xmlns:skos="http://www.w3.org/2004/02/skos/core#" rdf:about="http://inspire.ec.europa.eu/metadata-codelist/SpatialScope/regional">
    <skos:prefLabel xml:lang="en">Regional</skos:prefLabel>
    <skos:scopeNote xml:lang="en">The scope of the data set intends to cover the territory of one or several sub-national level administrative units.</skos:scopeNote>
    <skos:prefLabel xml:lang="bg">Регионално ниво</skos:prefLabel>
    <skos:scopeNote xml:lang="bg">Обхватът на набора от данни има за цел да покрие територията на една или няколко поднационални административни единици.</skos:scopeNote>
    <skos:prefLabel xml:lang="cs">Regionální</skos:prefLabel>
    <skos:scopeNote xml:lang="cs">Datová sada má v úmyslu pokrýt území jednoho nebo několika správních jednotek na nižší než celostátní úrovni.</skos:scopeNote>
    <skos:prefLabel xml:lang="hr">Regionalni</skos:prefLabel>
    <skos:scopeNote xml:lang="hr">Opseg skupa podataka namjerava se odnostiti na državno područje jedne ili više upravnih jedinica na podnacionalnoj razini.</skos:scopeNote>
    <skos:prefLabel xml:lang="da">Regionale</skos:prefLabel>
    <skos:scopeNote xml:lang="da">Formålet med datasættet er at dække et eller flere subnationale administrative niveauer i landet.</skos:scopeNote>
    <skos:prefLabel xml:lang="de">Regional</skos:prefLabel>
    <skos:scopeNote xml:lang="de">Der Geltungsbereich des Datensatzes deckt das Gebiet einer oder mehrerer Verwaltungseinheiten auf subnationaler Ebene ab.</skos:scopeNote>
    <skos:prefLabel xml:lang="el">Περιφερειακό</skos:prefLabel>
    <skos:scopeNote xml:lang="el">Το πεδίο εφαρμογής του συνόλου δεδομένων, έχει ως στόχο να καλύπτει την επικράτεια μιας ή περισσοτέρων διοικητικών μονάδων κατώτερων του εθνικού επιπέδου.</skos:scopeNote>
    <skos:prefLabel xml:lang="es">Regionales</skos:prefLabel>
    <skos:scopeNote xml:lang="es">El ámbito de aplicación del conjunto de datos se propone cubrir el territorio de una o varias unidades administrativas de nivel subnacional.</skos:scopeNote>
    <skos:prefLabel xml:lang="et">Piirkondlik</skos:prefLabel>
    <skos:scopeNote xml:lang="et">Andmekogumi eesmärk on hõlmata ühe või mitme riigi tasandist madalama tasandi haldusüksuse territooriumi.</skos:scopeNote>
    <skos:prefLabel xml:lang="fi">Alueellinen</skos:prefLabel>
    <skos:scopeNote xml:lang="fi">Tietoaineiston tarkoituksena on kattaa yhden tai useamman valtiotasoa alemman hallintotason hallintoyksikön alue.</skos:scopeNote>
    <skos:prefLabel xml:lang="fr">Régional</skos:prefLabel>
    <skos:scopeNote xml:lang="fr">Le champ d’application de la série de données vise à couvrir le territoire d’une ou de plusieurs unités administratives de niveau infranational.</skos:scopeNote>
    <skos:prefLabel xml:lang="hu">Regionális</skos:prefLabel>
    <skos:scopeNote xml:lang="hu">Az adatkészlet terjedelme egy vagy több, nemzetinél alacsonyabb szintű közigazgatási egység területét kívánja lefedni.</skos:scopeNote>
    <skos:prefLabel xml:lang="it">Regionale</skos:prefLabel>
    <skos:scopeNote xml:lang="it">L'ambito di applicazione dell'insieme di dati intende coprire il territorio di una o più unità amministrative di livello subnazionale.</skos:scopeNote>
    <skos:prefLabel xml:lang="lt">Regionų</skos:prefLabel>
    <skos:scopeNote xml:lang="lt">Duomenų rinkinio taikymo sritis apima vieno ar kelių subnacionalinio lygmens administracinių vienetų teritoriją.</skos:scopeNote>
    <skos:prefLabel xml:lang="lv">Reģionālā</skos:prefLabel>
    <skos:scopeNote xml:lang="lv">Datu kopas darbības joma ir paredzēta, lai aptvertu vienas vai vairāku vietējā līmeņa administratīvo vienību teritoriju.</skos:scopeNote>
    <skos:prefLabel xml:lang="mt">Reġjonali</skos:prefLabel>
    <skos:scopeNote xml:lang="mt">Il-kamp ta’ applikazzjoni ta’ sett ta’ dejta għandu l-għan li jkopri unitajiet amministrattivi ta’ livell subnazzjonali wieħed jew aktar.</skos:scopeNote>
    <skos:prefLabel xml:lang="nl">Regionaal</skos:prefLabel>
    <skos:scopeNote xml:lang="nl">De reikwijdte van de gegevensverzameling is bedoeld om het grondgebied van een of meer administratieve eenheden op subnationaal niveau te bestrijken.</skos:scopeNote>
    <skos:prefLabel xml:lang="pl">Regionalnym</skos:prefLabel>
    <skos:scopeNote xml:lang="pl">Zakres zbioru danych ma obejmować terytorium jednej lub kilku jednostek administracyjnych szczebla niższego niż krajowy.</skos:scopeNote>
    <skos:prefLabel xml:lang="pt">Regional</skos:prefLabel>
    <skos:scopeNote xml:lang="pt">O âmbito do conjunto de dados pretende abranger o território de uma ou mais unidades administrativas a nível subnacional.</skos:scopeNote>
    <skos:prefLabel xml:lang="ro">Regional</skos:prefLabel>
    <skos:scopeNote xml:lang="ro">Domeniul de aplicare al setului de date vizează acoperirea teritoriului uneia sau mai multor unități administrative de nivel sub-național.</skos:scopeNote>
    <skos:prefLabel xml:lang="sk">Regionálny</skos:prefLabel>
    <skos:scopeNote xml:lang="sk">Rozsah súboru priestorových údajov sa vzťahuje na jednu, alebo viaceré správne jednotky na nižšej ako celoštátnej úrovni.</skos:scopeNote>
    <skos:prefLabel xml:lang="sl">Regionalno</skos:prefLabel>
    <skos:scopeNote xml:lang="sl">Namen zbirke podatkov je zajeti ozemlje ene ali več upravnih enot na podnacionalni ravni.</skos:scopeNote>
    <skos:prefLabel xml:lang="sv">Regional</skos:prefLabel>
    <skos:scopeNote xml:lang="sv">Syftet med datamängden är att täcka en eller flera administrativa enheter på subnationell nivå.</skos:scopeNote>
    <skos:inScheme rdf:resource="http://inspire.ec.europa.eu/metadata-codelist/SpatialScope" />
  </skos:Concept>
  <skos:Concept xmlns:skos="http://www.w3.org/2004/02/skos/core#" rdf:about="http://inspire.ec.europa.eu/metadata-codelist/SpatialScope/local">
    <skos:prefLabel xml:lang="en">Local</skos:prefLabel>
    <skos:scopeNote xml:lang="en">The scope of the data set intends to cover the territory of one or several local administrative units.</skos:scopeNote>
    <skos:prefLabel xml:lang="bg">Местно ниво</skos:prefLabel>
    <skos:scopeNote xml:lang="bg">Обхватът на набора от данни има за цел да покрие територията на една или няколко местни административни единици.</skos:scopeNote>
    <skos:prefLabel xml:lang="cs">Místní</skos:prefLabel>
    <skos:scopeNote xml:lang="cs">Datová sada má v úmyslu pokrýt území jedné nebo několika místních správních jednotek.</skos:scopeNote>
    <skos:prefLabel xml:lang="hr">Lokalni</skos:prefLabel>
    <skos:scopeNote xml:lang="hr">Opseg skupa podataka namjerava se odnositi na područje jedne ili više lokalnih upravnih jedinica.</skos:scopeNote>
    <skos:prefLabel xml:lang="da">Lokal</skos:prefLabel>
    <skos:scopeNote xml:lang="da">Formålet med datasættet er at dække et eller flere lokale administrative niveauer i landet.</skos:scopeNote>
    <skos:prefLabel xml:lang="de">Lokal</skos:prefLabel>
    <skos:scopeNote xml:lang="de">Der Geltungsbereich des Datensatzes deckt das Gebiet einer oder mehrerer lokaler Verwaltungseinheiten ab.</skos:scopeNote>
    <skos:prefLabel xml:lang="el">Τοπικό</skos:prefLabel>
    <skos:scopeNote xml:lang="el">Το πεδίο εφαρμογής του συνόλου δεδομένων, έχει ως στόχο να καλύπτει την επικράτεια μιας ή περισσοτέρων τοπικών διοικητικών μονάδων.</skos:scopeNote>
    <skos:prefLabel xml:lang="es">Local</skos:prefLabel>
    <skos:scopeNote xml:lang="es">El ámbito de aplicación del conjunto de datos se propone cubrir el territorio de una o varias unidades administrativas locales.</skos:scopeNote>
    <skos:prefLabel xml:lang="et">Kohalik</skos:prefLabel>
    <skos:scopeNote xml:lang="et">Andmekogumi eesmärk on hõlmata ühe või mitme kohaliku haldusüksuse territooriumi.</skos:scopeNote>
    <skos:prefLabel xml:lang="fi">Paikallinen</skos:prefLabel>
    <skos:scopeNote xml:lang="fi">Tietoaineiston tarkoituksena on kattaa yhden tai useamman paikallisen hallintoyksikön alue.</skos:scopeNote>
    <skos:prefLabel xml:lang="fr">Local</skos:prefLabel>
    <skos:scopeNote xml:lang="fr">La portée de l’ensemble de données vise à couvrir le territoire d’une ou de plusieurs unités administratives locales.</skos:scopeNote>
    <skos:prefLabel xml:lang="hu">Helyi</skos:prefLabel>
    <skos:scopeNote xml:lang="hu">Az adatkészlet terjedelme egy vagy több helyi közigazgatási egység területét érinti.</skos:scopeNote>
    <skos:prefLabel xml:lang="it">Locale</skos:prefLabel>
    <skos:scopeNote xml:lang="it">L'ambito di applicazione dell'insieme di dati intende coprire il territorio di una o più unità amministrative locali.</skos:scopeNote>
    <skos:prefLabel xml:lang="lt">Vietos</skos:prefLabel>
    <skos:scopeNote xml:lang="lt">Duomenų rinkinio taikymo sritis apima vieno arba kelių vietos administracinių vienetų teritoriją.</skos:scopeNote>
    <skos:prefLabel xml:lang="lv">Vietējā</skos:prefLabel>
    <skos:scopeNote xml:lang="lv">Datu kopas darbības joma ir paredzēta, lai aptvertu vienas vai vairāku vietējo administratīvo vienību teritoriju.</skos:scopeNote>
    <skos:prefLabel xml:lang="mt">Lokali</skos:prefLabel>
    <skos:scopeNote xml:lang="mt">Il-kamp ta’ applikazzjoni tas-sett ta’ dejta għandu l-għan li jkopri t-territorju ta’ unità amministrattiva lokali waħda jew aktar.</skos:scopeNote>
    <skos:prefLabel xml:lang="nl">Lokaal</skos:prefLabel>
    <skos:scopeNote xml:lang="nl">De reikwijdte van de gegevensverzameling is bedoeld om het grondgebied van een of meer lokale administratieve eenheden te bestrijken.</skos:scopeNote>
    <skos:prefLabel xml:lang="pl">Lokalne</skos:prefLabel>
    <skos:scopeNote xml:lang="pl">Zakres zbioru danych ma obejmować terytorium jednej lub kilku lokalnych jednostek administracyjnych.</skos:scopeNote>
    <skos:prefLabel xml:lang="pt">Local</skos:prefLabel>
    <skos:scopeNote xml:lang="pt">O âmbito do conjunto de dados pretende abranger o território de uma ou várias unidades administrativas locais.</skos:scopeNote>
    <skos:prefLabel xml:lang="ro">Local</skos:prefLabel>
    <skos:scopeNote xml:lang="ro">Domeniul de aplicare al setului de date vizează acoperirea teritoriului uneia sau mai multor unități administrative locale.</skos:scopeNote>
    <skos:prefLabel xml:lang="sk">Miestny</skos:prefLabel>
    <skos:scopeNote xml:lang="sk">Rozsah súboru priestorových údajov sa vzťahuje na jednu, alebo viaceré miestne administratívne jednotky.</skos:scopeNote>
    <skos:prefLabel xml:lang="sl">Lokalno</skos:prefLabel>
    <skos:scopeNote xml:lang="sl">Namen zbirke podatkov je zajeti ozemlje ene ali več lokalnih upravnih enot.</skos:scopeNote>
    <skos:prefLabel xml:lang="sv">Lokal</skos:prefLabel>
    <skos:scopeNote xml:lang="sv">Syftet med datamängden är att täcka en eller flera lokala administrativa enheters territorium.</skos:scopeNote>
    <skos:inScheme rdf:resource="http://inspire.ec.europa.eu/metadata-codelist/SpatialScope" />
  </skos:Concept>
  <skos:Concept xmlns:skos="http://www.w3.org/2004/02/skos/core#" rdf:about="http://inspire.ec.europa.eu/metadata-codelist/SpatialScope/global">
    <skos:prefLabel xml:lang="en">Global</skos:prefLabel>
    <skos:scopeNote xml:lang="en">The scope of the data set intends to cover the whole Earth.</skos:scopeNote>
    <skos:prefLabel xml:lang="bg">Глобално ниво</skos:prefLabel>
    <skos:scopeNote xml:lang="bg">Обхватът на набора от данни има за цел да покрие цялата територия на Земята.</skos:scopeNote>
    <skos:prefLabel xml:lang="cs">Globální</skos:prefLabel>
    <skos:scopeNote xml:lang="cs">Datová sada má v úmyslu pokrýt celou Zemi.</skos:scopeNote>
    <skos:prefLabel xml:lang="hr">Globalni</skos:prefLabel>
    <skos:scopeNote xml:lang="hr">Opseg skupa podataka namjerava se odnositi na cijelu Zemlju.</skos:scopeNote>
    <skos:prefLabel xml:lang="da">Global</skos:prefLabel>
    <skos:scopeNote xml:lang="da">Formålet med datasættet er at dække hele Jorden.</skos:scopeNote>
    <skos:prefLabel xml:lang="de">Global</skos:prefLabel>
    <skos:scopeNote xml:lang="de">Der Geltungsbereich des Datensatzes deckt die gesamte Erde ab.</skos:scopeNote>
    <skos:prefLabel xml:lang="el">Παγκόσμιο</skos:prefLabel>
    <skos:scopeNote xml:lang="el">Το πεδίο εφαρμογής του συνόλου δεδομένων έχει ως στόχο να καλύπτει ολόκληρη τη Γη.</skos:scopeNote>
    <skos:prefLabel xml:lang="es">Global</skos:prefLabel>
    <skos:scopeNote xml:lang="es">El alcance del conjunto de datos se propone cubrir todo el planeta.</skos:scopeNote>
    <skos:prefLabel xml:lang="et">Üleilmne</skos:prefLabel>
    <skos:scopeNote xml:lang="et">Andmekogumi eesmärk on hõlmata kogu maailma.</skos:scopeNote>
    <skos:prefLabel xml:lang="fi">Maailmanlaajuinen</skos:prefLabel>
    <skos:scopeNote xml:lang="fi">Tietoaineiston tarkoituksena on kattaa koko maapallo.</skos:scopeNote>
    <skos:prefLabel xml:lang="fr">Mondial</skos:prefLabel>
    <skos:scopeNote xml:lang="fr">Le champ d’application de la série de données vise à couvrir l’ensemble de la Terre.</skos:scopeNote>
    <skos:prefLabel xml:lang="hu">Globális</skos:prefLabel>
    <skos:scopeNote xml:lang="hu">Az adathalmaznak a Föld egészére ki kell terjednie.</skos:scopeNote>
    <skos:prefLabel xml:lang="it">Globale</skos:prefLabel>
    <skos:scopeNote xml:lang="it">L'ambito di applicazione dell'insieme di dati intende coprire l'intera Terra.</skos:scopeNote>
    <skos:prefLabel xml:lang="lt">Pasaulinis</skos:prefLabel>
    <skos:scopeNote xml:lang="lt">Duomenų rinkinys skirtas visai Žemei.</skos:scopeNote>
    <skos:prefLabel xml:lang="lv">Globāls</skos:prefLabel>
    <skos:scopeNote xml:lang="lv">Datu kopas darbības joma ir paredzēta, lai aptvertu visu Zemi.</skos:scopeNote>
    <skos:prefLabel xml:lang="mt">Globali</skos:prefLabel>
    <skos:scopeNote xml:lang="mt">Il-kamp ta’ applikazzjoni tas-sett ta’ data għandu l-għan li jkopri d-Dinja kollha.</skos:scopeNote>
    <skos:prefLabel xml:lang="nl">Globaal</skos:prefLabel>
    <skos:scopeNote xml:lang="nl">De reikwijdte van de gegevensverzameling is bedoeld om de hele aarde te bestrijken.</skos:scopeNote>
    <skos:prefLabel xml:lang="pl">Globalny</skos:prefLabel>
    <skos:scopeNote xml:lang="pl">Zakres zbioru danych ma obejmować całą Ziemię.</skos:scopeNote>
    <skos:prefLabel xml:lang="pt">Mundial</skos:prefLabel>
    <skos:scopeNote xml:lang="pt">O âmbito do conjunto de dados pretende abranger toda a Terra.</skos:scopeNote>
    <skos:prefLabel xml:lang="ro">Mondial</skos:prefLabel>
    <skos:scopeNote xml:lang="ro">Domeniul de aplicare al setului de date vizează acoperirea întregului Pământ.</skos:scopeNote>
    <skos:prefLabel xml:lang="sk">Globálny</skos:prefLabel>
    <skos:scopeNote xml:lang="sk">Rozsah súboru priestorových údajov sa vzťahuje celú Zem.</skos:scopeNote>
    <skos:prefLabel xml:lang="sl">Globalno</skos:prefLabel>
    <skos:scopeNote xml:lang="sl">Namen zbirke podatkov je zajeti celotno Zemljo.</skos:scopeNote>
    <skos:prefLabel xml:lang="sv">Global</skos:prefLabel>
    <skos:scopeNote xml:lang="sv">Syftet med datamängden är att täcka hela jorden.</skos:scopeNote>
    <skos:inScheme rdf:resource="http://inspire.ec.europa.eu/metadata-codelist/SpatialScope" />
  </skos:Concept>
  <skos:Concept xmlns:skos="http://www.w3.org/2004/02/skos/core#" rdf:about="http://inspire.ec.europa.eu/metadata-codelist/SpatialScope/european">
    <skos:prefLabel xml:lang="en">European</skos:prefLabel>
    <skos:scopeNote xml:lang="en">The scope of the data set intends to cover Europe.</skos:scopeNote>
    <skos:prefLabel xml:lang="bg">Европейско ниво</skos:prefLabel>
    <skos:scopeNote xml:lang="bg">Обхватът на набора от данни има за цел да обхване Европа.</skos:scopeNote>
    <skos:prefLabel xml:lang="cs">Evropská</skos:prefLabel>
    <skos:scopeNote xml:lang="cs">Datová sada má v úmyslu pokrýt Evropu.</skos:scopeNote>
    <skos:prefLabel xml:lang="hr">Europski</skos:prefLabel>
    <skos:scopeNote xml:lang="hr">Opseg skupa podataka namjerava se odnositi na Europu.</skos:scopeNote>
    <skos:prefLabel xml:lang="da">Europæiske</skos:prefLabel>
    <skos:scopeNote xml:lang="da">Formålet med datasættet er at dække hele Europa.</skos:scopeNote>
    <skos:prefLabel xml:lang="de">Europäisch</skos:prefLabel>
    <skos:scopeNote xml:lang="de">Der Geltungsbereich des Datensatzes deckt Europa ab.</skos:scopeNote>
    <skos:prefLabel xml:lang="el">Ευρωπαϊκό</skos:prefLabel>
    <skos:scopeNote xml:lang="el">Το πεδίο εφαρμογής του συνόλου δεδομένων έχει ως στόχο να καλύπτει την Ευρώπη.</skos:scopeNote>
    <skos:prefLabel xml:lang="es">Europea</skos:prefLabel>
    <skos:scopeNote xml:lang="es">El ámbito de aplicación del conjunto de datos se propone cubrir Europa.</skos:scopeNote>
    <skos:prefLabel xml:lang="et">Euroopa</skos:prefLabel>
    <skos:scopeNote xml:lang="et">Andmekogumi eesmärk on hõlmata Euroopat.</skos:scopeNote>
    <skos:prefLabel xml:lang="fi">Eurooppalainen</skos:prefLabel>
    <skos:scopeNote xml:lang="fi">Tietoaineiston tarkoituksena on kattaa Eurooppa.</skos:scopeNote>
    <skos:prefLabel xml:lang="fr">Européen</skos:prefLabel>
    <skos:scopeNote xml:lang="fr">Le champ d’application de la série de données vise à couvrir l’Europe.</skos:scopeNote>
    <skos:prefLabel xml:lang="hu">Európai</skos:prefLabel>
    <skos:scopeNote xml:lang="hu">A kitűzött adatok köre az Európára is ki fog terjedni.</skos:scopeNote>
    <skos:prefLabel xml:lang="it">Europeo</skos:prefLabel>
    <skos:scopeNote xml:lang="it">L'ambito di applicazione del set di dati intende coprire l'Europa.</skos:scopeNote>
    <skos:prefLabel xml:lang="lt">Europos</skos:prefLabel>
    <skos:scopeNote xml:lang="lt">Duomenų rinkinio paskirtis – apimti Europą.</skos:scopeNote>
    <skos:prefLabel xml:lang="lv">Eiropas</skos:prefLabel>
    <skos:scopeNote xml:lang="lv">Datu kopas darbības joma ir paredzēta, lai aptvertu Eiropu.</skos:scopeNote>
    <skos:prefLabel xml:lang="mt">Ewropea</skos:prefLabel>
    <skos:scopeNote xml:lang="mt">Il-kamp ta’ applikazzjoni tas-sett ta’ data għandu l-għan li jkopri l-Ewropa.</skos:scopeNote>
    <skos:prefLabel xml:lang="nl">Europees</skos:prefLabel>
    <skos:scopeNote xml:lang="nl">De reikwijdte van de gegevensverzameling is bedoeld voor Europa.</skos:scopeNote>
    <skos:prefLabel xml:lang="pl">Europejska</skos:prefLabel>
    <skos:scopeNote xml:lang="pl">Zakres zbioru danych ma obejmować Europę.</skos:scopeNote>
    <skos:prefLabel xml:lang="pt">Europeia</skos:prefLabel>
    <skos:scopeNote xml:lang="pt">O âmbito do conjunto de dados pretende abranger a Europa.</skos:scopeNote>
    <skos:prefLabel xml:lang="ro">European</skos:prefLabel>
    <skos:scopeNote xml:lang="ro">Domeniul de aplicare al setului de date vizează acoperirea Europei.</skos:scopeNote>
    <skos:prefLabel xml:lang="sk">Európsky</skos:prefLabel>
    <skos:scopeNote xml:lang="sk">Rozsah súboru priestorových údajov sa vzťahuje na Európu.</skos:scopeNote>
    <skos:prefLabel xml:lang="sl">Evropsko</skos:prefLabel>
    <skos:scopeNote xml:lang="sl">Namen zbirke podatkov je zajeti Evropo.</skos:scopeNote>
    <skos:prefLabel xml:lang="sv">Europeisk</skos:prefLabel>
    <skos:scopeNote xml:lang="sv">Syftet med datamängden är att omfatta Europa.</skos:scopeNote>
    <skos:inScheme rdf:resource="http://inspire.ec.europa.eu/metadata-codelist/SpatialScope" />
  </skos:Concept>
</rdf:RDF>

